Moving negotiation functionality from Handshake module

src/tls/Handshake.fst
@@ -47,8 +47,7 @@ let prepareClientHello cfg ks log ri sido =
 	 None) in
   let sid = (match sido with | None -> empty_bytes | Some x -> x) in
   let ci = initConnection Client cr in
-  let ext = prepareExtensions cfg ci ri kp in
-  let co = prepareClientOffer cfg in
+  let co = prepareClientOffer cfg ci ri kp in
   let ch = 
   {ch_protocol_version = co.co_protocol_version;
    ch_client_random = cr;
@@ -56,7 +55,7 @@ let prepareClientHello cfg ks log ri sido =
    ch_cipher_suites = co.co_cipher_suites;
    ch_raw_cipher_suites = None;
    ch_compressions = co.co_compressions;
-   ch_extensions = Some ext;} in
+   ch_extensions = co.co_extensions;} in
   let chb = log @@ (ClientHello ch) in
   (ClientHello ch, chb)
 
@@ -82,49 +81,12 @@ let gte_pv_geqPV pv1 pv2 = ()
 
 (* Returns [c] if [c] is within the range of acceptable versions for [cfg],
  * [Error] otherwise. *)
-val negotiateVersion: cfg:config -> c:protocolVersion -> Tot (result protocolVersion)
-let negotiateVersion cfg c =
-  if geqPV c cfg.minVer && geqPV cfg.maxVer c then Correct c
-  else if geqPV c cfg.maxVer then Correct cfg.maxVer
-  else Error(AD_internal_error, perror __SOURCE_FILE__ __LINE__ "Protocol version negotiation failed")
-
-val negotiate:l1:list valid_cipher_suite -> list valid_cipher_suite -> Tot (option (c:valid_cipher_suite{is_CipherSuite c && List.Tot.mem c l1}))
-let negotiate l1 l2 =
-  List.Tot.find #valid_cipher_suite (fun s -> is_CipherSuite s && List.Tot.mem s l1) l2
-
-val negotiateCipherSuite: cfg:config -> pv:protocolVersion -> c:valid_cipher_suites -> Tot (result (TLSConstants.kexAlg * option TLSConstants.sigAlg * TLSConstants.aeAlg * valid_cipher_suite))
-let negotiateCipherSuite cfg pv c =
-  match negotiate c cfg.ciphersuites with
-  | Some(CipherSuite kex sa ae) -> Correct(kex,sa,ae,CipherSuite kex sa ae)
-  | None -> Error(AD_internal_error, perror __SOURCE_FILE__ __LINE__ "Cipher suite negotiation failed")
 
 // TODO : IMPLEMENT
 val getCachedSession: cfg:config -> ch:ch -> ST (option session)
   (requires (fun h -> True))
   (ensures (fun h0 i h1 -> True))
 let getCachedSession cfg cg = None
-
-// FIXME: no FFDHE, doesn't check cfg.namedGroups
-val negotiateGroupKeyShare: config -> protocolVersion -> kexAlg -> option (list extension) -> Tot (result (namedGroup * option bytes))
-let rec negotiateGroupKeyShare cfg pv kex exts =
-  match exts with
-  | None ->
-    begin
-    match pv,kex with
-    | TLS_1p2, Kex_ECDHE -> Correct (SEC ECC_P256, None)
-    | _ -> Error(AD_decode_error, "no supported group or key share extension found")
-    end
-  | Some exts ->
-    begin
-    let rec aux: config -> protocolVersion -> kexAlg -> list extension -> Tot (result (namedGroup * option bytes)) = fun cfg pv kex es ->
-      match pv,kex,es with
-      | TLS_1p3, Kex_ECDHE, E_keyShare (ClientKeyShare ((gn,gxb)::_)) :: _ ->
-	Correct (gn,Some gxb)
-      | TLS_1p3,_, h::t -> aux cfg pv kex t
-      | _ -> Error(AD_decode_error, "no supported group or key share extension found")
-    in
-    aux cfg pv kex exts
-    end
 
 #set-options "--lax"
 
@@ -133,93 +95,62 @@ val prepareServerHello: config -> KeySchedule.ks -> HandshakeLog.log -> option r
   (requires (fun h -> True))
   (ensures (fun h0 i h1 -> True))
 let prepareServerHello cfg ks log ri (ClientHello ch,_) =
-  match negotiateVersion cfg ch.ch_protocol_version with
-    | Error(z) -> Error(z)
-    | Correct(pv) ->
-  match negotiateCipherSuite cfg pv ch.ch_cipher_suites with
-    | Error(z) -> Error(z)
-    | Correct(kex,sa,ae,cs) ->
-  match negotiateGroupKeyShare cfg pv kex ch.ch_extensions with
-    | Error(z) -> Error(z)
-    | Correct(gn,gxo) ->
+ let mode_wo_ext = computeServerMode cfg ch.ch_protocol_version ch.ch_cipher_suites ch.ch_extensions ch.ch_compressions in  
+  match mode_wo_ext with
+   | Error(z) -> Error(z)
+   | Correct(mode_wo_ext) ->
+
   let srand = KeySchedule.ks_server_random ks in
   let ksl = 
-    (match pv,gxo with
-     | TLS_1p3,Some gxb -> 
-       let gyb = KeySchedule.ks_server_13_1rtt_init ks ch.ch_client_random cs gn gxb in
+    (match mode_wo_ext.sm_protocol_version, mode_wo_ext.sm_dh_group, mode_wo_ext.sm_dh_share with
+     | TLS_1p3, Some gn, Some gxb -> 
+       let gyb = KeySchedule.ks_server_13_1rtt_init ks ch.ch_client_random mode_wo_ext.sm_cipher_suite gn gxb in
        (Some (ServerKeyShare (gn,gyb)))
-    | _ -> None) in
-  match negotiateServerExtensions pv ch.ch_extensions ch.ch_cipher_suites cfg cs ri ksl false with
+     | _ -> None) in
+  match updateServerMode cfg mode_wo_ext ch.ch_extensions ch.ch_cipher_suites ri ksl with
     | Error(z) -> Error(z)
-    | Correct(sext,next) ->
-    let sid = CoreCrypto.random 32 in
-    let comp = match ch.ch_compressions with
-      | [] -> None
-      | _ -> Some NullCompression in
-    let sh = 
-      {sh_protocol_version = pv;
-       sh_sessionID = Some sid;
-       sh_server_random = srand;
-       sh_cipher_suite = cs;
-       sh_compression = comp;
-       sh_extensions = sext} in
-    let nego = 
-      {n_client_random = ch.ch_client_random;
-       n_server_random = srand;
-       n_sessionID = Some sid;
-       n_protocol_version = pv;
-       n_kexAlg = kex;
-       n_sigAlg = sa;
-       n_aeAlg  = ae;
-       n_cipher_suite = cs;
-       n_compression = comp;
-       n_dh_group = Some gn;
-       n_scsv = [];
-       n_extensions = next;
-       (* [getCachedSession] returned [None], so no session resumption *)
-       n_resume = false} in
-    let _ = log @@ (ClientHello ch) in
-    let shb = log @@ (ServerHello sh) in
-    let lb = HandshakeLog.getHash log in
-    let keys = (match pv with
+    | Correct(sext,next,mode) ->
+
+//let (sext, mode) = updateServerMode cfg mode_wo_ext ch.ch_extensions ch.ch_cipher_suites ri ksl in
+//    match (sext, mode) with
+//     | Error(z) -> Error(z)
+//     | Correct(sext,mode) ->
+//  match negotiateServerExtensions mode.sm_protocol_version ch.ch_extensions ch.ch_cipher_suites cfg mode.sm_cipher_suite ri ksl false with
+//  | Error(z) -> Error(z)
+//   | Correct(sext,next) ->
+  let sid = CoreCrypto.random 32 in
+  let sh = 
+   {sh_protocol_version = mode.sm_protocol_version;
+    sh_sessionID = Some sid;
+    sh_server_random = srand;
+    sh_cipher_suite = mode.sm_cipher_suite;
+    sh_compression = mode.sm_comp;
+    sh_extensions = sext} in
+  let nego = 
+   {n_client_random = ch.ch_client_random;
+    n_server_random = srand;
+    n_sessionID = Some sid;
+    n_protocol_version = mode.sm_protocol_version;
+    n_kexAlg = mode.sm_kexAlg;
+    n_sigAlg = mode.sm_sigAlg;
+    n_aeAlg  = mode.sm_aeAlg;
+    n_cipher_suite = mode.sm_cipher_suite;
+    n_compression = mode.sm_comp;
+    n_dh_group = mode.sm_dh_group;
+    n_scsv = [];
+    n_extensions = next;
+    (* [getCachedSession] returned [None], so no session resumption *)
+    n_resume = false} in
+  let _ = log @@ (ClientHello ch) in
+  let shb = log @@ (ServerHello sh) in
+  let lb = HandshakeLog.getHash log in
+  let keys = (match mode.sm_protocol_version with
     	     | TLS_1p3 -> 
 	       let keys = KeySchedule.ks_server_13_get_htk ks lb  in
 	       Some keys
 	     | _ -> None) in
     Correct (nego,keys,(ServerHello sh,shb))
 
-(* Is this one of the special random values indicated by the RFC (6.3.1.1)? *)
-val isSentinelRandomValue: protocolVersion -> protocolVersion -> TLSInfo.random -> Tot bool
-let isSentinelRandomValue c_pv s_pv s_random =
-  geqPV c_pv TLS_1p3 && geqPV TLS_1p2 s_pv && equalBytes (abytes "DOWNGRD\x01") s_random ||
-  geqPV c_pv TLS_1p2 && geqPV TLS_1p1 s_pv && equalBytes (abytes "DOWNGRD\x00") s_random
-
-(* If [true], then:
-  - both the client and server versions are within the range specified by [cfg]
-  - the server is not newer than the client
-  - there is no undesired downgrade (as indicated by the special random values).
-*)
-val acceptableVersion: config -> ch -> protocolVersion -> TLSInfo.random -> Tot bool
-let acceptableVersion cfg ch s_pv s_random =
-  match negotiateVersion cfg ch.ch_protocol_version with
-  | Correct c_pv -> 
-    geqPV c_pv s_pv && geqPV s_pv cfg.minVer &&
-    not (isSentinelRandomValue c_pv s_pv s_random)
-  | Error _ ->
-    false
-
-(* If [true], then:
-  - [s_cs] is has been offered previously;
-  - [s_cs] is consistent with the [config];
-  - TODO: [s_cs] is supported by the protocol version (e.g. no GCM with
-    TLS<1.2).
-*)
-val acceptableCipherSuite: config -> ch -> protocolVersion -> valid_cipher_suite -> Tot bool
-let acceptableCipherSuite cfg ch s_pv s_cs =
-  // JP: I would think the first line implies the second one?
-  List.Tot.existsb (fun x -> x = s_cs) ch.ch_cipher_suites &&
-  List.Tot.existsb (fun x -> x = s_cs) cfg.ciphersuites &&
-  not (isAnonCipherSuite s_cs) || cfg.allowAnonCipherSuite
   
 val processServerHello: c:config -> KeySchedule.ks -> HandshakeLog.log -> option ri -> ch -> (hs_msg * bytes) ->
   ST (result (nego * option KeySchedule.recordInstance))
@@ -227,45 +158,36 @@ val processServerHello: c:config -> KeySchedule.ks -> HandshakeLog.log -> option
      (ensures (fun h0 i h1 -> True))
 let processServerHello cfg ks log ri ch (ServerHello sh,_) =
   let _ = log @@ (ServerHello sh) in
-  // Assuming no resumption; TODO: add it 
-  if not (acceptableVersion cfg ch sh.sh_protocol_version sh.sh_server_random) then
-    Error(AD_illegal_parameter, perror __SOURCE_FILE__ __LINE__ "Protocol version negotiation")
-  else  if not (acceptableCipherSuite cfg ch sh.sh_protocol_version sh.sh_cipher_suite) then
-    Error(AD_illegal_parameter, perror __SOURCE_FILE__ __LINE__ "Ciphersuite negotiation")
-  else
-  let resume = false in
-  match negotiateClientExtensions sh.sh_protocol_version cfg ch.ch_extensions sh.sh_extensions sh.sh_cipher_suite ri resume with
-    | Error z -> Error z
-    | Correct next -> 
-        match sh.sh_cipher_suite with
-	| CipherSuite kex sa ae ->
-        let o_nego = 
-          {n_client_random = ch.ch_client_random;
-           n_server_random = sh.sh_server_random;
-           n_sessionID = sh.sh_sessionID;
-           n_protocol_version = sh.sh_protocol_version;
-           n_kexAlg = kex;
-           n_aeAlg = ae;
-	   n_sigAlg = sa;
-           n_cipher_suite = sh.sh_cipher_suite;
-	   n_dh_group = None;
-           n_compression = sh.sh_compression;
-	   n_scsv = [];
-           n_extensions = next;
-           n_resume = false } in
-	   (match sh.sh_protocol_version, kex, next.ne_keyShare with
-	    | TLS_1p3, Kex_DHE, Some (gn,gyb) 
-	    | TLS_1p3, Kex_ECDHE, Some (gn,gyb) -> 
-	      	   let lb = HandshakeLog.getHash log in
+  let mode = computeClientMode cfg ch.ch_extensions ch.ch_protocol_version sh.sh_protocol_version sh.sh_server_random sh.sh_cipher_suite sh.sh_extensions sh.sh_compression ri in
+   match mode with
+    | Error(z) -> Error(z)
+    | Correct(mode) ->  
+   let o_nego = 
+    {n_client_random = ch.ch_client_random;
+     n_server_random = sh.sh_server_random;
+     n_sessionID = sh.sh_sessionID;
+     n_protocol_version = mode.cm_protocol_version;
+     n_kexAlg = mode.cm_kexAlg;
+     n_aeAlg = mode.cm_aeAlg;
+     n_sigAlg = mode.cm_sigAlg;
+     n_cipher_suite = mode.cm_cipher_suite;
+     n_dh_group = mode.cm_dh_group;
+     n_compression = sh.sh_compression;
+     n_scsv = [];
+     n_extensions = mode.cm_ext;
+     n_resume = false } in
+    (match o_nego.n_protocol_version, o_nego.n_kexAlg, mode.cm_dh_group, mode.cm_dh_share with
+     | TLS_1p3, Kex_DHE, Some gn, Some gyb 
+     | TLS_1p3, Kex_ECDHE, Some gn, Some gyb -> 
+    	   let lb = HandshakeLog.getHash log in
 	           let keys = KeySchedule.ks_client_13_1rtt ks o_nego.n_cipher_suite (gn, gyb) lb in
 	      	   Correct (o_nego,Some keys)
-            | _ -> Correct (o_nego,None))
-	| _ -> Error (AD_decode_error, "ServerHello CipherSuite not a real ciphersuite")
-
+     | _ -> Correct (o_nego,None))
+    
 #reset-options
 
 (* Handshake API: TYPES, taken from FSTI *)
-
+ 
 type clientState = 
   | C_Idle:                  option ri -> clientState
   | C_HelloSent:        option ri -> ch -> clientState
@@ -379,7 +301,6 @@ let latest h (s:hs{Seq.length (logT s h) > 0}) = // accessing the latest epoch
 (*   forall_epochs s h0 (fun e ->  *)
 (*     let rs = regions e in  *)
 (*     (forall (r:rid{Set.mem r rs}).{:pattern (Set.mem r rs)} Map.sel h0 r = Map.sel h1 r)) *)
-
 
 // separation policy: the handshake mutates its private state, 
 // only depends on it, and only extends the log with fresh epochs.
