src/tls/Negotiation.fst
@@ -15,6 +15,38 @@ open CoreCrypto
 (* Negotiation: HELLO sub-module *)
 type ri = cVerifyData * sVerifyData 
 
+type clientOffer = {
+  co_protocol_version:protocolVersion;
+  co_cipher_suites:(k:valid_cipher_suites{List.Tot.length k < 256});
+  co_compressions:(cl:list compression{List.Tot.length cl > 0 /\ List.Tot.length cl < 256});
+  co_extensions:option (ce:list extension{List.Tot.length ce < 256});
+}
+
+type serverMode = {
+     sm_protocol_version: protocolVersion;
+     sm_kexAlg: TLSConstants.kexAlg;
+     sm_aeAlg: TLSConstants.aeAlg;
+     sm_sigAlg: option TLSConstants.sigAlg;
+     sm_cipher_suite: cipherSuite;
+     sm_dh_group: option namedGroup;
+     sm_dh_share: option bytes;
+     sm_comp: option compression;
+     sm_ext: option negotiatedExtensions;
+}
+
+type clientMode = {
+     cm_protocol_version: protocolVersion;
+     cm_kexAlg: TLSConstants.kexAlg;
+     cm_aeAlg: TLSConstants.aeAlg;
+     cm_sigAlg: option TLSConstants.sigAlg;
+     cm_cipher_suite: cipherSuite;
+     cm_dh_group: option namedGroup;
+     cm_dh_share: option bytes;
+     cm_comp: option compression;
+     cm_ext: negotiatedExtensions;
+}
+
+
 type nego = {
      n_resume: bool;
      n_client_random: TLSInfo.random;
@@ -29,6 +61,7 @@ type nego = {
      n_compression: option compression;
      n_extensions: negotiatedExtensions;
      n_scsv: list scsv_suite;
+     
 }                 
 
 type hs_id = {
@@ -57,22 +90,189 @@ val handshakeId: handshake -> Tot id
 
 let handshakeId h = noId // Placeholder 
 
-type clientOffer = {
-  co_protocol_version:protocolVersion;
-  co_cipher_suites:(k:valid_cipher_suites{List.Tot.length k < 256});
-  co_compressions:(cl:list compression{List.Tot.length cl > 0 /\ List.Tot.length cl < 256});
- // co_extensions:option (ce:list extension{List.Tot.length ce < 256});
-}
-
-val prepareClientOffer: config -> Tot clientOffer
-let prepareClientOffer cfg =
+val prepareClientOffer: cfg:config -> ci:connectionInfo -> ri:option (cVerifyData *sVerifyData) -> kp: option keyShare -> Tot clientOffer
+let prepareClientOffer cfg ci ri kp =
+  let ext = prepareExtensions cfg ci ri kp in
   let co = 
   {co_protocol_version = cfg.maxVer;
    co_cipher_suites = cfg.ciphersuites;
    co_raw_cipher_suites = None;
    co_compressions = [NullCompression];
+   co_extensions = Some ext;
    } in
   co
- // let ext = prepareExtensions cfg ci ri kp in 
- // MK: ignoring extensions for now as we don't have ci ...
- //  co_extensions = Some ext;} in
+
+// Checks that the protocol version in the CHELO message is
+// within the range of versions supported by the server configuration
+// and outputs the negotiated version if true
+val negotiateVersion: cfg:config -> c:protocolVersion -> Tot (result protocolVersion)
+let negotiateVersion cfg c =
+  if geqPV c cfg.minVer && geqPV cfg.maxVer c then Correct c
+  else if geqPV c cfg.maxVer then Correct cfg.maxVer
+  else Error(AD_internal_error, perror __SOURCE_FILE__ __LINE__ "Protocol version negotiation failed")
+
+// For use in negotiating the ciphersuite, takes two lists and
+// outputs the first ciphersuite in list2 that also is in list
+// one and is a valid ciphersuite, or [None]
+val negotiate:l1:list valid_cipher_suite -> list valid_cipher_suite -> Tot (option (c:valid_cipher_suite{is_CipherSuite c && List.Tot.mem c l1}))
+let negotiate l1 l2 =
+  List.Tot.find #valid_cipher_suite (fun s -> is_CipherSuite s && List.Tot.mem s l1) l2
+
+// For use in ensuring the result from negotiate is a Correct
+// ciphersuite with associated kex, sig and ae algorithms,
+// and throws an error if No ciphersuites were supported in both lists
+val negotiateCipherSuite: cfg:config -> pv:protocolVersion -> ccs:valid_cipher_suites -> Tot (result (TLSConstants.kexAlg * option TLSConstants.sigAlg * TLSConstants.aeAlg * valid_cipher_suite))
+let negotiateCipherSuite cfg pv ccs =
+  match negotiate ccs cfg.ciphersuites with
+  | Some(CipherSuite kex sa ae) -> Correct(kex,sa,ae,CipherSuite kex sa ae)
+  | None -> Error(AD_internal_error, perror __SOURCE_FILE__ __LINE__ "Cipher suite negotiation failed")
+
+// FIXME: no FFDHE, doesn't check cfg.namedGroups
+val negotiateGroupKeyShare: config -> protocolVersion -> kexAlg -> option (list extension) -> Tot (result (namedGroup * option bytes))
+let rec negotiateGroupKeyShare cfg pv kex exts =
+  match exts with
+  | None ->
+    begin
+    match pv,kex with
+    | TLS_1p2, Kex_ECDHE -> Correct (SEC ECC_P256, None)
+    | _ -> Error(AD_decode_error, "no supported group or key share extension found")
+    end
+  | Some exts ->
+    begin
+    let rec aux: config -> protocolVersion -> kexAlg -> list extension -> Tot (result (namedGroup * option bytes)) = fun cfg pv kex es ->
+      match pv,kex,es with
+      | TLS_1p3, Kex_ECDHE, E_keyShare (ClientKeyShare ((gn,gxb)::_)) :: _ ->
+        Correct (gn,Some gxb)
+      | TLS_1p3,_, h::t -> aux cfg pv kex t
+      | _ -> Error(AD_decode_error, "no supported group or key share extension found")
+    in
+    aux cfg pv kex exts
+    end
+
+// Determines if the server random value contains a downgrade flag
+// AND if there has been a downgrade
+// The downgrade flag is a random value set by RFC (6.3.1.1)
+val isSentinelRandomValue: protocolVersion -> protocolVersion -> TLSInfo.random -> Tot bool
+let isSentinelRandomValue c_pv s_pv s_random =
+  geqPV c_pv TLS_1p3 && geqPV TLS_1p2 s_pv && equalBytes (abytes "DOWNGRD\x01") s_random ||
+  geqPV c_pv TLS_1p2 && geqPV TLS_1p1 s_pv && equalBytes (abytes "DOWNGRD\x00") s_random
+
+// Confirms that the version negotiated by the server was:
+// - within the range specified by client config AND
+// - is not an unnecessary downgrade AND
+// - is not a newer version than offered by the client 
+
+val acceptableVersion: config -> protocolVersion -> protocolVersion -> TLSInfo.random -> Tot bool
+let acceptableVersion cfg cpv spv sr =
+  match negotiateVersion cfg cpv with
+  | Correct c_pv ->
+    geqPV c_pv spv && geqPV spv cfg.minVer &&
+    not (isSentinelRandomValue c_pv spv sr)
+  | Error _ ->
+    false
+
+// Confirms that the ciphersuite negotiated by the server was:
+//  - consistent with the client config;
+//  - TODO: [s_cs] is supported by the protocol version (e.g. no GCM with
+//    TLS<1.2).
+// BD: Removed that the ciphersuite is acceptable given CHELO
+// given that the clientOffer is prepared with the entire list
+// of valid cipher suites in the client config
+val acceptableCipherSuite: config -> protocolVersion -> valid_cipher_suite -> Tot bool
+let acceptableCipherSuite cfg spv cs =
+  List.Tot.existsb (fun x -> x = cs) cfg.ciphersuites &&
+  not (isAnonCipherSuite cs) || cfg.allowAnonCipherSuite
+
+// TODO BD: ignoring extensions for the moment
+// due to the fact that we require calling the keyschedule
+// in between negotiating the named Group and preparing the
+// negotiated Extensions
+val computeServerMode: cfg:config -> cpv:protocolVersion -> ccs:valid_cipher_suites -> cexts:option (list extension) -> comps: (list compression) -> Tot (result serverMode)
+ let computeServerMode cfg cpv ccs cexts comps = 
+  (match (negotiateVersion cfg cpv) with 
+    | Error(z) -> Error(z)
+    | Correct(npv) -> 
+  match negotiateCipherSuite cfg npv ccs with
+    | Error(z) -> Error(z)
+    | Correct(kex,sa,ae,cs) ->
+  match negotiateGroupKeyShare cfg npv kex cexts with
+    | Error(z) -> Error(z)
+    | Correct(gn,gxo) ->
+  let comp = match comps with
+    | [] -> None
+    | _ -> Some NullCompression in
+  let mode =
+    {sm_protocol_version = npv;
+     sm_kexAlg = kex;
+     sm_aeAlg = ae;
+     sm_sigAlg = sa;
+     sm_cipher_suite = cs;
+     sm_dh_group = Some gn;
+     sm_dh_share = gxo;
+     sm_comp = comp;
+     sm_ext = None;
+    } in
+  Correct (mode))
+
+val updateServerMode: cfg:config -> sm:serverMode -> cexts:option (list extension) -> ccs:valid_cipher_suites -> ri:option (cVerifyData *sVerifyData) -> kp: option keyShare -> Tot (result (option (list extension) * negotiatedExtensions * serverMode))
+let updateServerMode cfg sm cexts ccs ri kp =
+  (match negotiateServerExtensions sm.sm_protocol_version cexts ccs cfg sm.sm_cipher_suite ri kp false with
+   | Error(z) -> Error(z)
+   | Correct(sext,next) ->
+  let mode =
+   {sm_protocol_version = sm.sm_protocol_version;
+    sm_kexAlg = sm.sm_kexAlg;
+    sm_aeAlg = sm.sm_aeAlg;
+    sm_sigAlg = sm.sm_sigAlg;
+    sm_cipher_suite = sm.sm_cipher_suite;
+    sm_dh_group = sm.sm_dh_group;
+    sm_dh_share = sm.sm_dh_share;
+    sm_comp = sm.sm_comp;
+    sm_ext = Some next;
+   } in
+  Correct (sext, next, mode))
+
+
+
+val computeClientMode: cfg:config -> cext:option (list extension) -> cpv:protocolVersion -> spv:protocolVersion -> sr:TLSInfo.random -> cs:valid_cipher_suite -> sext:option (list extension) -> comp:option compression -> option ri -> Tot (result clientMode)
+let computeClientMode cfg cext cpv spv sr cs sext comp ri =
+  if not (acceptableVersion cfg cpv spv sr) then
+    Error(AD_illegal_parameter, perror __SOURCE_FILE__ __LINE__ "Protocol version negotiation")
+  else if not (acceptableCipherSuite cfg spv cs) then
+    Error(AD_illegal_parameter, perror __SOURCE_FILE__ __LINE__ "Ciphersuite negotiation")
+  else
+   let resume = false in
+   match negotiateClientExtensions spv cfg cext sext cs ri resume with
+    | Error(z) -> Error(z)
+    | Correct(next) ->
+    match cs with
+     | CipherSuite kex sa ae ->
+      match spv, kex, next.ne_keyShare with
+       | TLS_1p3, Kex_DHE, Some (gn, gyb)
+       | TLS_1p3, Kex_ECDHE, Some (gn, gyb) ->
+         let mode =
+         {cm_protocol_version = spv;
+          cm_kexAlg = kex;
+          cm_aeAlg = ae;
+          cm_sigAlg = sa;
+          cm_cipher_suite = cs;
+          cm_dh_group = Some gn;
+          cm_dh_share = Some gyb;
+          cm_comp = comp;
+          cm_ext = next;
+         } in
+         Correct(mode)
+       | _ ->
+         let mode =
+         {cm_protocol_version = spv;
+          cm_kexAlg = kex;
+          cm_aeAlg = ae;
+          cm_sigAlg = sa;
+          cm_cipher_suite = cs;
+          cm_dh_group = None;
+          cm_dh_share = None;
+          cm_comp = comp;
+          cm_ext = next;
+         } in
+         Correct(mode)
+      | _ -> Error (AD_decode_error, "ServerHello ciphersuite is not a real ciphersuite")
